triple as record + triple_inj definition

src/Triple.v
@@ -1,77 +1,116 @@
+From mathcomp Require Import all_ssreflect.
+Set Implicit Arguments.
+Unset Strict Implicit.
+Unset Printing Implicit Defensive.
 From RDF Require Import Term.
-From Coq Require Import Lists.ListSet.
-From Coq Require Import Init.Nat.
-From Coq Require Import Strings.String.
-From Coq Require Import Bool.Bool.
-
-Inductive trpl : Type :=
-  | triple (s p o : term).
-
-Record tripl_r : Set := mkTrpl
-                       { the_triple : trpl
-                      }. 
 
 
-Definition proj_subject (t : trpl) : term :=
-  match t with
-  | triple s _ _ => s
-  end.
-Definition proj_predicate (t : trpl) : term :=
-  match t with
-  | triple _ p _ => p
-  end.
+Section Triple.
 
-Definition proj_object (t : trpl) : term :=
-  match t with
-  | triple _ _ o => o
-  end.
+  Variable I B L: eqType.
+  (* Notation "t.s" := (proj_subject t) (at level X) (* which scope? *) *)
+  Let term:= (term I B L).
+  Let is_iri:= (@is_iri I B L).
+  Let is_bnode:= (@is_bnode I B L).
+  Let is_lit:= (@is_lit I B L).
 
-(* alias for triple of terms type *)
-(* Definition triple := (node * term * term)%type.  *)
+  (* Inductive trpl : Type := *)
+  (* | triple (s p o : term). *)
 
-(*
-   Inductive rdf : Type :=
-  | graph (triples : list triple).
- *)
+  (* Definition proj_subject (t : trpl) : term := *)
+  (*   match t with *)
+  (*   | triple s _ _ => s *)
+  (*   end. *)
 
-Definition app_μ_to_triple (μ : term -> term) (t : trpl) : trpl:=
-  (match t with
-   | (triple n1 n2 n3) => triple (μ n1) n2 (μ n3)
-   end).
+  (* Definition proj_predicate (t : trpl) : term := *)
+  (*   match t with *)
+  (*   | triple _ p _ => p *)
+  (*   end. *)
 
-Definition eqb_triple (t1 t2:trpl) : bool :=
-  (match t1,t2 with
-   | (triple s p o),(triple s2 p2 o2) => (eqb_term s s2) && (eqb_term p p2) && (eqb_term o o2)
-   end).
+  (* Definition proj_object (t : trpl) : term := *)
+  (*   match t with *)
+  (*   | triple _ _ o => o *)
+  (*   end. *)
 
-Theorem eqb_eq_triple: forall (t1 t2 : trpl),
-  eqb_triple t1 t2 = true <-> t1 = t2.
-Proof. intros. split; intros H.
-  - destruct t1,t2 as [s2 p2 o2]; f_equal;
-    simpl in H; apply andb_true_iff in H; destruct H as [H0 H2]; apply andb_true_iff in H0; destruct H0 as [H H1]; apply eqb_eq_term. 
-    + apply H.
-    + apply H1.
-    + apply H2.
-  - destruct t1,t2 as [s2 p2 o2]. injection H as H1 H2 H3. simpl. rewrite H1. rewrite H2. rewrite H3.
-    rewrite (eqb_term_refl s2). rewrite (eqb_term_refl p2). rewrite (eqb_term_refl o2). reflexivity.
-Qed.
+  (* Definition part_in (t : trpl) (part : trpl -> term) (is_in : term -> bool) : bool := *)
+  (*   is_in (part t). *)
 
-Theorem eqb_triple_refl : forall (t1: trpl),
-  eqb_triple t1 t1 = true.
-Proof. intros. destruct t1. simpl. rewrite (eqb_term_refl s). rewrite (eqb_term_refl p). rewrite (eqb_term_refl o). reflexivity.
-Qed.
+  (* Definition subject_in_ib (t : trpl) : bool := *)
+  (*   part_in t proj_subject (fun trm => is_iri trm || is_bnode trm). *)
 
-Theorem eqb_neq_triple : forall (t1 t2: trpl),
-  eqb_triple t1 t2 = false <-> t1 <> t2.
-Proof. intros. split.
-  - intros H contra. rewrite contra in H. rewrite eqb_triple_refl in H. discriminate H.
-  - intros H. unfold not in H. rewrite <- eqb_eq_triple in H. destruct (eqb_triple t1 t2).
-    + exfalso. apply H. reflexivity.
-    + reflexivity.
-Qed.
+  (* Definition predicate_in_i (t : trpl) : bool := *)
+  (*   part_in t proj_predicate is_iri. *)
 
-Theorem eq_dec_triple : forall (t1 t2: trpl),
-  {t1 = t2} + {t1 <> t2}.
-Proof. decide equality; try decide equality; try apply string_dec; decide equality. Qed.
+  (* Definition object_in_ibl (t : trpl) : bool := *)
+  (*   part_in t proj_object (fun trm => is_iri trm || is_bnode trm || is_lit trm). *)
 
-(* Notation "t.s" := ( f α) (at level 20, α at next level) : selection_scope. *)
+  Record triple := mkTriple { subject : term
+                           ; predicate : term
+                           ; object: term
+                           ; subject_in_IB: is_iri subject || is_bnode subject == true
+                           ; predicate_in_I: is_iri predicate == true
+                           ; object_in_IBL: is_iri object || is_bnode object || is_lit object == true
+                        }. 
+
+  Lemma tripl_inj : forall (t1 t2: triple),
+      subject t1 = subject t2 ->
+      predicate t1 = predicate t2 ->
+      object t1 = object t2 ->
+      t1 = t2.
+  Proof. move=> [s1 p1 o1 sin1 pin1 oin1] [s2 p2 o2 sin2 pin2 oin2] /= seq peq oeq.
+         (* rewrite /subject /predicate /object /=. *)
+         (* rewrite seq. *)
+         (* apply: val. rewrite seq. (eq_irrelevance bool). *)
+  Admitted.
+
+  (* alias for triple of terms type *)
+  (* Definition triple := (node * term * term)%type.  *)
+
+  (*
+    Inductive rdf : Type :=
+    | graph (triples : list triple).
+  *)
+
+  (* Definition image (t : triple) (μ : B -> B) : triple := *)
+  (*   let (s,p,o,sin,pin,oin) := t in *)
+  (*   {μ s,μ p,μ o,sin,pin,oin}. *)
+
+
+
+
+  (* Definition eqb_triple (t1 t2:trpl) : bool := *)
+  (*   (match t1,t2 with *)
+  (*   | (triple s p o),(triple s2 p2 o2) => (eqb_term s s2) && (eqb_term p p2) && (eqb_term o o2) *)
+  (*   end). *)
+
+  (* Theorem eqb_eq_triple: forall (t1 t2 : trpl), *)
+  (*   eqb_triple t1 t2 = true <-> t1 = t2. *)
+  (* Proof. intros. split; intros H. *)
+  (*   - destruct t1,t2 as [s2 p2 o2]; f_equal; *)
+  (*     simpl in H; apply andb_true_iff in H; destruct H as [H0 H2]; apply andb_true_iff in H0; destruct H0 as [H H1]; apply eqb_eq_term.  *)
+  (*     + apply H. *)
+  (*     + apply H1. *)
+  (*     + apply H2. *)
+  (*   - destruct t1,t2 as [s2 p2 o2]. injection H as H1 H2 H3. simpl. rewrite H1. rewrite H2. rewrite H3. *)
+  (*     rewrite (eqb_term_refl s2). rewrite (eqb_term_refl p2). rewrite (eqb_term_refl o2). reflexivity. *)
+  (* Qed. *)
+
+  (* Theorem eqb_triple_refl : forall (t1: trpl), *)
+  (*   eqb_triple t1 t1 = true. *)
+  (* Proof. intros. destruct t1. simpl. rewrite (eqb_term_refl s). rewrite (eqb_term_refl p). rewrite (eqb_term_refl o). reflexivity. *)
+  (* Qed. *)
+
+  (* Theorem eqb_neq_triple : forall (t1 t2: trpl), *)
+  (*   eqb_triple t1 t2 = false <-> t1 <> t2. *)
+  (* Proof. intros. split. *)
+  (*   - intros H contra. rewrite contra in H. rewrite eqb_triple_refl in H. discriminate H. *)
+  (*   - intros H. unfold not in H. rewrite <- eqb_eq_triple in H. destruct (eqb_triple t1 t2). *)
+  (*     + exfalso. apply H. reflexivity. *)
+  (*     + reflexivity. *)
+  (* Qed. *)
+
+  (* Theorem eq_dec_triple : forall (t1 t2: trpl), *)
+  (*   {t1 = t2} + {t1 <> t2}. *)
+  (* Proof. decide equality; try decide equality; try apply string_dec; decide equality. Qed. *)
+
+End Triple.
